# imports: http://purl.bdrc.io/ontology/admin/

@prefix : <http://purl.bdrc.io/ontology/ext/auth/> .
@prefix adm: <http://purl.bdrc.io/ontology/admin/> .
@prefix adr: <http://purl.bdrc.io/resource-nc/auth/> .
@prefix aut: <http://purl.bdrc.io/ontology/ext/auth/> .
@prefix bda: <http://purl.bdrc.io/admindata/> .
@prefix bdo: <http://purl.bdrc.io/ontology/core/> .
@prefix bdr: <http://purl.bdrc.io/resource/> .
@prefix dct: <http://purl.org/dc/terms/> .
@prefix foaf: <http://xmlns.com/foaf/0.1/> .
@prefix owl: <http://www.w3.org/2002/07/owl#> .
@prefix rdf: <http://www.w3.org/1999/02/22-rdf-syntax-ns#> .
@prefix rdfs: <http://www.w3.org/2000/01/rdf-schema#> .
@prefix xsd: <http://www.w3.org/2001/XMLSchema#> .

<http://purl.bdrc.io/ontology/ext/auth/>
	a owl:Ontology ;
	rdfs:label "Buda authentication ontology"@en ;
	dct:license bda:LicenseCC0 ;
	owl:imports <http://purl.bdrc.io/ontology/admin/> ;
	.

aut:Application
	a owl:Class ;
	rdfs:subClassOf aut:Entity ;
	rdfs:label "application"@en ;
	rdfs:comment "represent a application that provides a set of web services or exposes endpoints. For instance, bdrc  Linked Data server is one app and bdrc IIIF Image server is another one."@en ;
	.

aut:AuthId
	a rdfs:Datatype ;
	owl:equivalentClass xsd:string ;
	.

aut:Endpoint
	a owl:Class ;
	rdfs:subClassOf aut:Entity ;
	rdfs:label "endpoint"@en ;
	rdfs:comment """The Endpoint object represents any secured web or REST service provided accross the whole organization. Endpoints are associated with a given app (Linked data server, Image server, etc...).
Any application implementing bdrc auth0 security can therefore filter its own secured endpoints and check against user credentials to allow or deny access to these endpoints."""@en ;
	.

aut:Entity
	a owl:Class ;
	.

aut:Group
	a owl:Class ;
	rdfs:subClassOf aut:Entity ;
	rdfs:label "group"@en ;
	rdfs:comment """The Group objects represent a specific category of users. 
Following auth0 model, Groups are also associated with roles, i.e that each member of the group inherits the roles associated with that group. 
Therefore, the role associated to a specific user are of two types: 
1) Specific roles associated with the user outside of a group; 
2) Roles inherited from all groups (and eventuelly nested groups) the user may belong to."""@en ;
	.

aut:Permission
	a owl:Class ;
	rdfs:subClassOf aut:Entity ;
	rdfs:label "permission"@en ;
	rdfs:comment """The Permission object represent fine grained authorization policies. It may be associated with a Role object and is therefore restricted to the application associated with that role.
For instance, a permission associated to bdrc Linked Data Server application can only be associated to a role defined for that same Linked Data server app."""@en ;
	.

aut:ResourceAccess
	a owl:Class ;
	rdfs:subClassOf aut:Entity ;
	rdfs:label "resource access"@en ;
	rdfs:comment "The ResourceAccess object defines a mapping between Permissions and bdrc AccessType. The auth mechanism looks for a match between User permissions and the specific AccessType of a requested resource."@en ;
	.

aut:Role
	a owl:Class ;
	rdfs:subClassOf aut:Entity ;
	rdfs:label "role"@en ;
	rdfs:comment """A Role object is associated to an application and possibly various Permission objects.
It is important to notice that roles are used for application level access control while groups can be used accross all applications."""@en ;
	.

aut:Subscriber
	a owl:Class ;
	rdfs:subClassOf aut:Entity ;
	rdfs:label "subscriber"@en ;
	rdfs:comment "A Subscribing institution, can be composed of multiple organizations (campus, library, office, etc.)."@en ;
	.

aut:SubscriberOrganization
	a owl:Class ;
	rdfs:subClassOf aut:Subscriber ;
	rdfs:label "subscriber organization"@en ;
	rdfs:comment "A distinct part of a subscribing institution"@en ;
	.

aut:UserProfile
	a owl:Class ;
	rdfs:subClassOf
		aut:Entity ,
		foaf:Agent
		;
	rdfs:label "user profile"@en ;
	rdfs:comment """The UserProfile object represents any person registered to the system. A user may belong to a Group and may have a Role.
It is worth noticing that permissions are not associated directly to a User but instead, through its various roles."""@en ;
	.

aut:appId
	a owl:ObjectProperty ;
	rdfs:label "application ID"@en ;
	rdfs:comment "This property links permissions, roles and endpoints to their associated application resources."@en ;
	rdfs:domain
		aut:Endpoint ,
		aut:Permission ,
		aut:Role
		;
	rdfs:range aut:Application ;
	.

aut:authId
	a owl:DatatypeProperty ;
	rdfs:label "authentification id"@en ;
	rdfs:comment "The unique id given to the user by the authorization provider"@en ;
	rdfs:domain aut:UserProfile ;
	rdfs:range xsd:string ;
	.

aut:created_at
	a owl:DatatypeProperty ;
	rdfs:label "creation date"@en ;
	rdfs:comment "The creation date of the auth0 user bdrc account"@en ;
	rdfs:domain aut:UserProfile ;
	rdfs:range xsd:dateTime ;
	.

aut:desc
	a owl:DatatypeProperty ;
	rdfs:label "description"@en ;
	rdfs:comment "A group, Role or Permission description"@en ;
	rdfs:domain
		aut:Application ,
		aut:Group ,
		aut:Permission ,
		aut:Role
		;
	rdfs:range rdf:PlainLiteral ;
	.

aut:forAnyStatus
	a owl:DatatypeProperty ;
	rdfs:label "is for any status"@en ;
	rdfs:comment "set the permission to get access to any resource, regardless the status, for all the users of a given group"@en ;
	rdfs:domain aut:Group ;
	rdfs:range xsd:boolean ;
	.

aut:forGroup
	a owl:ObjectProperty ;
	rdfs:label "for group"@en ;
	rdfs:comment "Besides linking a UserProfile to the groups he belongs to, this property also links a specific endpoint to its authorized groups resources."@en ;
	rdfs:domain
		aut:Endpoint ,
		aut:UserProfile
		;
	rdfs:range aut:Group ;
	.

aut:forPermission
	a owl:ObjectProperty ;
	rdfs:label "for permission"@en ;
	rdfs:comment "Links ResourceAccess and Endpoints to the required permissions resources. This is used in bdrc specific auth model (i.e ResourceAccess and Endpoints are not modelizations of auth0 objects)."@en ;
	rdfs:domain
		aut:Endpoint ,
		aut:ResourceAccess
		;
	rdfs:range aut:Permission ;
	.

aut:forRole
	a owl:ObjectProperty ;
	rdfs:label "for role"@en ;
	rdfs:comment """Links Endpoints to their authorized auth0 roles, allowing request filters to give or deny access to endpoints according to a specific user profile. 
Note that this property also links Endpoints (implicitly) to permissions associated to auth0 corresponding roles"""@en ;
	rdfs:domain aut:Endpoint ;
	rdfs:range aut:Role ;
	.

aut:hasIPAddress
	a owl:DatatypeProperty ;
	rdfs:label "IP addresses"@en ;
	rdfs:comment "An IP address associated with an organization, can contain a subnet mask"@en ;
	rdfs:domain aut:Subscriber ;
	rdfs:range xsd:string ;
	.

aut:hasMember
	a owl:ObjectProperty ;
	rdfs:label "has member"@en ;
	rdfs:comment "Links Users and Groups following auth0 model"@en ;
	rdfs:domain aut:Group ;
	rdfs:range aut:UserProfile ;
	.

aut:hasPermission
	a owl:ObjectProperty ;
	rdfs:label "has permission"@en ;
	rdfs:comment "Links Roles and permissions, following Auth0 model."@en ;
	rdfs:domain aut:Role ;
	rdfs:range aut:Permission ;
	.

aut:hasRole
	a owl:ObjectProperty ;
	rdfs:comment
		"Links Groups or Users to Roles, following auth0 model."@en ,
		"has role"@en
		;
	rdfs:domain
		aut:Group ,
		aut:UserProfile
		;
	rdfs:range aut:Role ;
	.

aut:last_login
	a owl:DatatypeProperty ;
	rdfs:label "last login time"@en ;
	rdfs:comment "The last login time and date of the auth0 user bdrc account"@en ;
	rdfs:domain aut:UserProfile ;
	rdfs:range xsd:dateTime ;
	.

aut:path
	a owl:DatatypeProperty ;
	rdfs:label "path"@en ;
	rdfs:comment """The unique path of a given Endpoint or web service. This path is unique for the application associated with this Endpoint.
Important: note that other endpoints of different applications may have the same path."""@en ;
	rdfs:domain aut:Endpoint ;
	rdfs:range xsd:string ;
	.

aut:personalAccess
	a owl:ObjectProperty ;
	rdfs:label "personal access"@en ;
	rdfs:comment "A resource Id based access authorization"@en ;
	rdfs:domain aut:UserProfile ;
	.

aut:policy
	a owl:ObjectProperty ;
	rdfs:label "policy"@en ;
	rdfs:comment """Links ResourceAccess objects to bdrc AccessType.
This property is used for checking access rights against protected resources available at secured or open endpoints. It corresponds to the finest grained authorization in bdrc auth implementation."""@en ;
	rdfs:domain aut:ResourceAccess ;
	rdfs:range adm:Access ;
	.

aut:subscribedTo
	a owl:ObjectProperty ;
	rdfs:label "subscribed to"@en ;
	rdfs:comment "What the subscriber subscribed to (usually a bdo:Collection)"@en ;
	rdfs:domain aut:Subscriber ;
	.

aut:updated_at
	a owl:DatatypeProperty ;
	rdfs:label "last update time"@en ;
	rdfs:comment "The last update time and date of the auth0 user bdrc account"@en ;
	rdfs:domain aut:UserProfile ;
	rdfs:range xsd:dateTime ;
	.

